Progress on Blake2s stateful code with Marina

code/hash/Hacl.Impl.Blake2s.fst
@@ -57,11 +57,15 @@ val update_sub: #a:Type0 -> #len:size_nat -> #olen:size_nat -> i:lbuffer a len -
   Stack unit
     (requires (fun h -> live h i /\ live h o))
     (ensures  (fun h0 _ h1 -> preserves_live h0 h1 /\ modifies1 i h0 h1
+                         /\ h0.[o] == h1.[o]
                          /\ h1.[i] == Spec.Lib.IntSeq.update_sub #a #len h0.[i] (v start) (v n) h0.[o]))
 
 let update_sub #a #len #olen i start n o =
+  let h0 = ST.get () in
   let i' = sub i start n in
-  copy n o i'
+  copy n o i';
+  let h1 = ST.get () in
+  assume(h0.[o] == h1.[o])
 
 
 ///
@@ -77,7 +81,7 @@ let size_hash_state : size_nat = 8
 type init_vector = lbuffer uint32 8
 type working_vector = lbuffer uint32 16
 type message_block = lbuffer uint32 16
-type hash_state = lbuffer uint32 size_hash_state
+type hash_state = lbuffer uint32 8
 type idx = n:size_t{size_v n < 16}
 type sigma_t = lbuffer (n:size_t{size_v n < 16}) 160
 
@@ -184,14 +188,34 @@ val blake2_compress1 : wv:working_vector ->
   s:hash_state -> m:message_block ->
   offset:uint64 -> flag:Spec.last_block_flag -> const_iv:lbuffer uint32 8 ->
   Stack unit
-    (requires (fun h -> live h s /\ live h m /\ live h wv /\ live h const_iv))
+    (requires (fun h -> live h s /\ live h m /\ live h wv /\ live h const_iv
+                   /\ as_list h.[const_iv] == Spec.list_init))
     (ensures  (fun h0 _ h1 -> preserves_live h0 h1
                          /\ modifies1 wv h0 h1
                          /\ h1.[wv] == Spec.Blake2s.blake2_compress1 h0.[wv] h0.[s] h0.[m] offset flag))
 
 let blake2_compress1 wv s m offset flag const_iv =
+  let h0 = ST.get () in
   update_sub wv (size 0) (size 8) s;
+  let h1 = ST.get () in
+  let v0 = normalize_term (v (size 0)) in
+  let v8 = normalize_term (v (size 8)) in
+  assume(h1.[const_iv] == h0.[const_iv]);
+  assume(h1.[m] == h0.[m]);
+  assert(h1.[s] == h0.[s]);
+  assert(live h1 wv);
+  assert(h1.[wv] == Spec.Lib.IntSeq.update_sub h0.[wv] (v (size 0)) 8 h0.[s]);
   update_sub wv (size 8) (size 8) const_iv;
+  let h2 = ST.get () in
+  assume(h2.[const_iv] == h1.[const_iv]);
+  assume(h2.[m] == h1.[m]);
+  assume(h2.[s] == h1.[s]);
+  assert(h2.[const_iv] == h0.[const_iv]);
+  assert(h2.[m] == h0.[m]);
+  assert(h2.[s] == h0.[s]);
+  assert(h2.[wv] == Spec.Lib.IntSeq.update_sub h1.[wv] v8 v8 h1.[const_iv]);
+  assert(h2.[wv] == Spec.Lib.IntSeq.update_sub (Spec.Lib.IntSeq.update_sub h0.[wv] v0 v8 h0.[s]) v8 v8 h1.[const_iv]);
+  //assert(Spec.Blake2s.blake2_compress1 h0.[wv] h0.[s] h0.[m] offset flag == Spec.Lib.IntSeq.update_sub (Spec.Lib.IntSeq.update_sub h0.[wv] v0 v8 h0.[s]) v8 v8 h1.[const_iv]);
   let low_offset = to_u32 #U64 offset in
   let high_offset = to_u32 #U64 (offset >>. u32 Spec.word_size) in
   let wv_12 = logxor #U32 wv.(size 12) low_offset in
@@ -199,7 +223,8 @@ let blake2_compress1 wv s m offset flag const_iv =
   let wv_14 = logxor #U32 wv.(size 14) (u32 0xFFFFFFFF) in
   wv.(size 12) <- wv_12;
   wv.(size 13) <- wv_13;
-  (if flag then wv.(size 14) <- wv_14)
+ (if flag then wv.(size 14) <- wv_14);
+ admit()
 
 
 val blake2_compress2 :
